lib/Maps.dfy
@@ -135,4 +135,11 @@ module Maps {
 	function MapToImap<K,V>(m: map<K,V>) : imap<K,V> {
 	  imap k | k in m :: m[k]
 	}
+
+	lemma IsMapUnion<K,V>(m1: map<K,V>, m2: map<K,V>, m: map<K,V>)
+	requires m1 !! m2
+	requires forall key | key in m1 :: key in m && m[key] == m1[key]
+	requires forall key | key in m2 :: key in m && m[key] == m2[key]
+	requires forall key | key in m :: (key in m1 || key in m2)
+	ensures m == MapUnion(m1, m2)
 }
